update proof

rocq/theories/verification.v
@@ -42,34 +42,29 @@ Definition trace_prefixes {A : Type} : Type := @trace (@trace A * A).
 
 
 
-Parameter input output mem : Type.
+Parameter input output state : Type.
 
 
 Abbreviation input_trace := (@trace input).
 Abbreviation output_trace := (@trace output). 
-Abbreviation mem_trace := (@trace mem). 
+Abbreviation state_trace := (@trace state). 
 
 
 
 (* 
-    given a new input i and with current memory mem, the program produced the output o
-    the new memory correspond to the next element in the list.
-
-    last output is the first element of the list
-
     an element ((i,m)(o,m')) of a trace represent the memory m' and output o produced by the program after receiving input i and memory m
 
-    invariant : m must be the same as previous m'
+    invariant : for a valid run, m must be the same as previous m'
 *)
-Definition pgrm_trace : Type := @trace ((input*mem)*(output*mem)). 
+Definition pgrm_trace : Type := @trace ((input*state)*(output*state)). 
 
-Definition pgrm_trace_split : pgrm_trace -> (input_trace * mem_trace) * (output_trace * mem_trace)  := fun tr =>
+Definition pgrm_trace_split : pgrm_trace -> (input_trace * state_trace) * (output_trace * state_trace)  := fun tr =>
     (List.split (fst (List.split tr)), List.split (snd (List.split tr))).
 
-Definition private_to_input_trace : pgrm_trace -> input_trace := fun tr =>  
+Definition trace_to_input_trace : pgrm_trace -> input_trace := fun tr =>  
     fst (fst (pgrm_trace_split tr)).
 
-Definition pgrm_trace_combine : (input_trace * mem_trace) * (output_trace * mem_trace) -> pgrm_trace := fun '((i,m),(o,m')) =>
+Definition pgrm_trace_combine : (input_trace * state_trace) * (output_trace * state_trace) -> pgrm_trace := fun '((i,m),(o,m')) =>
     List.combine (List.combine i m) (List.combine o m').
 
 Fact pgrm_trace_split_cons tr i o m m' : 
@@ -127,7 +122,7 @@ Proof.
         destruct (split im) eqn:Hbla; destruct (split om') eqn:Hbla'; cbn; subst. now inversion Heq_om'. 
 Qed.
 
-Lemma combine_split_trace (i_t: input_trace) (m_t m_t': mem_trace) (o_t : output_trace) :
+Lemma combine_split_trace (i_t: input_trace) (m_t m_t': state_trace) (o_t : output_trace) :
     List.length i_t = List.length m_t /\
     List.length m_t = List.length m_t'/\
     List.length o_t = List.length m_t 
@@ -197,18 +192,18 @@ Proof.
     - now rewrite IHtr at 1 2.
 Qed.
 
-Definition f : Type := input * mem -> output * mem.
+Definition f : Type := input * state -> output * state.
 
 Record Program : Type := {
-    setup: unit -> mem;
+    setup: state;
     loop: f;
 }.
 
-(* run m l is the trace produced by the program where m is the first memory state  *)
+(* run P l is the trace produced by executing the program P *)
 Inductive run (P : Program) : pgrm_trace -> Prop :=
     | run_start i o m' : 
-        loop P (i,(setup P tt)) = (o,m') ->
-        run P (((i,(setup P tt)),(o,m'))::nil)
+        loop P (i,setup P) = (o,m') ->
+        run P (((i,setup P),(o,m'))::nil)
     
     | run_next tr prev_i prev_o prev_m i o m m' : 
         run P (((prev_i, prev_m), (prev_o, m))::tr) ->
@@ -224,9 +219,9 @@ Proof.
     intros H. now inversion H.
 Qed.
 
-(* property made up of the history of previous inputs, states and outputs and current input and mem *)
-Definition local_precond : Type :=  pgrm_trace -> (input*mem) -> Prop.
-Definition local_postcond : Type :=  pgrm_trace -> (input*mem) -> (output*mem) -> Prop.
+(* property made up of the history of previous inputs, states and outputs and current input and state *)
+Definition local_precond : Type :=  pgrm_trace -> (input*state) -> Prop.
+Definition local_postcond : Type :=  pgrm_trace -> (input*state) -> (output*state) -> Prop.
 
 
 
@@ -245,20 +240,15 @@ Definition valid_triple (T:HoareTriple) tr i m o m' : Prop :=
 .
 
 
-Definition aut_complete {N L} (a: automaton N L): Prop := 
-    forall n, reachable a n -> exists p m, transition a n p m.
-
-
 (* 'assumes' automata transition label: predicate on previous inputs and current input *)
 Definition a_aut_label : Type := @trace input -> input -> Prop.
 
 Definition sat_a (p: a_aut_label) '((t,i): @trace input * input) : Prop := p t i.
 
-
 (* 'guarantees' automata transition label: predicate on trace history, current input and memory, and next output and memory  *)
-Definition g_aut_label : Type :=  pgrm_trace -> (input*mem) -> (output*mem) -> Prop.
+Definition g_aut_label : Type :=  pgrm_trace -> (input*state) -> (output*state) -> Prop.
 
-Definition sat_g (p: g_aut_label) '((t,(im,om')): @pgrm_trace * ((input * mem) * (output * mem))) : Prop :=
+Definition sat_g (p: g_aut_label) '((t,(im,om')): @pgrm_trace * ((input * state) * (output * state))) : Prop :=
     p t im om'.
 
 
@@ -269,7 +259,7 @@ Parameter g_aut_node : Type.
 
 (* hardy's input: temporal contracts defined as büchi automata *)
 Record Contract : Type := {
-    contract_setup : mem -> Prop;
+    contract_setup : state -> Prop;
     contract_assumes : automaton a_aut_node a_aut_label;
     contract_guarantees : automaton g_aut_node g_aut_label;
 }.
@@ -277,14 +267,58 @@ Record Contract : Type := {
 
 (* given a stream of inputs accepted by a_aut, the program always produces a stream of outputs accepted by g_aut *)
 Definition valid_contract (C: Contract) (P: Program): Prop := 
-    (contract_setup C) (setup P tt) ->
-    forall t, 
-    run P t ->
-    forall i_t m_t o_t,
-    (i_t,m_t,o_t) = pgrm_trace_split t ->
+    (contract_setup C) (setup P) ->
+    forall tr, run P tr ->
+    forall i_t m_t o_t,  (i_t,m_t,o_t) = pgrm_trace_split tr ->
     language sat_a (contract_assumes C) (build_trace_history i_t) -> 
-    language sat_g (contract_guarantees C) (build_trace_history t)
+    language sat_g (contract_guarantees C) (build_trace_history tr)
 .
+
+
+Definition aut_complete {N L} (a: automaton N L): Prop := 
+    forall n, reachable a n -> exists p m, transition a n p m.
+
+Lemma prod_complete {N1 N2 L1 L2} (a: automaton N1 L1) (b : automaton N2 L2) : 
+    aut_complete a -> 
+    aut_complete b ->
+    aut_complete (product a b).
+Proof.
+    intros * Ha Hb n H.
+    assert (reachable a (fst n)).
+    {
+        destruct n.
+        simpl.
+        apply reachable_left_proj in H.
+        apply H.
+    }
+    assert (reachable b (snd n)).
+    {
+        destruct n.
+        apply reachable_right_proj in H.  
+        apply H.
+    }
+    apply Ha in H0 as [f [n1 Hat]].
+    apply Hb in H1 as [g [m1 Hbt]].
+    exists (f,g), (n1,m1).
+    split; assumption.
+Qed.
+
+
+Definition aut_deterministic {N L A} (a: automaton N L) (belongs : L -> A -> Prop) : Prop := 
+    forall w p p', 
+    language_wit belongs a p w ->
+    language_wit belongs a p' w ->
+    p = p'
+.
+
+
+Lemma prod_deterministic {N1 N2 L1 L2 A B} (a: automaton N1 L1) (b : automaton N2 L2) (a_belongs : L1 -> A -> Prop) (b_belongs : L2 -> B -> Prop): 
+    aut_deterministic a a_belongs ->
+    aut_deterministic b b_belongs ->
+    aut_deterministic (product a b) (fun '(x,y) '(a,b) => a_belongs x a /\ b_belongs y b).
+Proof.
+Admitted.
+
 
 
 Section Reduction.
@@ -295,82 +329,107 @@ Section Reduction.
     Definition g_aut := contract_guarantees C.
 
 
+
+    (* Lemma aut_deterministic_local_choice {N L A} (a: automaton N L) (belongs : L -> A -> Prop)  : 
+        aut_deterministic a belongs ->
+        forall w n m m' p p',
+
+        exists p, path atm (init atm) p /\ 
+                valid (List.map fst p) w.
+                
+                
+        valid belongs p w ->
+        transition a n p m ->
+        transition a n p' m' -> 
+        p = p'
+    . *)
+
+
+    
+
     Parameter a_aut_complete : aut_complete a_aut.
     Parameter g_aut_complete : aut_complete g_aut.
 
+    Parameter a_aut_deterministic : aut_deterministic a_aut sat_a.
+    Parameter g_aut_deterministic  : aut_deterministic g_aut sat_g.
     
     Abbreviation ag_aut_node := (a_aut_node * g_aut_node)%type.
     Abbreviation ag_aut_label  := (a_aut_label * g_aut_label)%type.
 
     Definition ag_aut : automaton ag_aut_node ag_aut_label := product (contract_assumes C) (contract_guarantees C).
 
-    Definition sat_ag (l: ag_aut_label) '((t,((i,m),(o,m'))): @pgrm_trace * ((input * mem) * (output * mem))): Prop :=
-        sat_a (fst l) (private_to_input_trace t,i) /\ 
+    Fact ag_aut_complete : aut_complete ag_aut.
+    Proof.
+        apply prod_complete; [exact a_aut_complete| exact g_aut_complete].
+    Qed.
+
+
+    Definition sat_ag (l: ag_aut_label) '((t,((i,m),(o,m'))): @pgrm_trace * ((input * state) * (output * state))): Prop :=
+        sat_a (fst l) (trace_to_input_trace t,i) /\ 
         sat_g (snd l) (t,((i,m),(o,m')))
     .
 
 
-    Lemma ag_aut_complete : 
-        forall n, reachable ag_aut n -> 
-            exists g m, transition ag_aut n g m.
-    Proof.
-        intros.
-        assert (reachable_from (contract_assumes C) (init (contract_assumes C)) (fst n)).
-        {
-            destruct n.
-            simpl.
-            apply reachable_left_proj in H.
-            apply H.
-        }
-        assert (reachable_from g_aut (init g_aut) (snd n)).
-        {
-            destruct n.
-            apply reachable_right_proj in H.  
-            apply H.
-        }
-        apply a_aut_complete in H0 as [f [n1 Ha]].
-        apply g_aut_complete in H1 as [g [m1 Hb]].
-        exists (f,g), (n1,m1).
-        split; assumption.
-    Qed.
+
 
     (* converts a postcondition for instant n into a precondition for instant n+1  *)
     Definition postcond_to_precond (post: local_postcond) : local_precond := fun t => match t with
     | nil => fun _ => True (* no history *)
-    | prev_inst::h =>  fun _ => 
+    | prev_inst::h =>  
+        fun _ => (* we discard current instant as the postcondition cannot mention it *)
         post h (fst (fst prev_inst), snd (fst prev_inst)) (fst (snd prev_inst), snd (snd prev_inst))
     end.
 
     (* disjunction of all predecesssors postcondition as precondition *)
-    Inductive join_preds (a: automaton ag_aut_node ag_aut_label) tr i m : ag_aut_node -> Prop :=
+    Inductive join_preds tr i m : ag_aut_node -> Prop :=
     | join_preds_setup :
         tr = nil /\ contract_setup C m ->
-        join_preds a tr i m (init a) 
+        join_preds tr i m (init ag_aut) 
 
     | join_preds_cons prev_n precond curr_n : 
-        predecessor _ _ a prev_n precond curr_n -> 
+        predecessor _ _ ag_aut prev_n precond curr_n -> 
         postcond_to_precond (snd precond) tr (i,m) ->
-        join_preds a tr i m curr_n
+        join_preds tr i m curr_n
+    .  
+
+    (* join_succs n pre tr i m o m' is the disjunction of all successors (pre',post) with a precondition equivalent to pre such post tr i m o m' *)
+    Inductive join_succs curr_node pre tr i m o m' : Prop := 
+    | join_succs_ pre' post' next_n  :
+        successor _ _ ag_aut next_n (pre',post') curr_node ->
+        pre' (trace_to_input_trace tr) i <-> pre (trace_to_input_trace tr) i ->
+        post' tr (i,m) (o,m') ->
+        join_succs curr_node pre tr i m o m'
     .  
 
 
-    Inductive triple_gen (a: automaton ag_aut_node ag_aut_label) (t: HoareTriple) n pre post tr i m o m' : Prop := 
-    | triple_gen__cons :
+    (* triple_gen t n pre tr i m o m' is the triple t generated for node n for the given precondition *)
+    Inductive triple_gen (t: HoareTriple) curr_node pre tr i m o m' : Prop := 
+    | triple_gen_cons :
+        
+        
         (* the triple precondition must be equivalent to the conjunction of the disjunction of previous postconditions and current precondition *)
-        (local_pre t tr (i,m) <-> (join_preds a tr i m n /\ pre (private_to_input_trace tr) i)) -> 
-        (local_post t tr (i,m) (o,m') <-> post tr (i,m) (o,m'))  ->
+        (   local_pre t tr (i,m) 
+            <-> 
+            (join_preds tr i m curr_node /\ pre (trace_to_input_trace tr) i)
+        ) 
+        ->
+        
+        (* the triple postcondition is the disjunction of all postconditions of successors nodes with equivalent precondition  *)
+        (
+            local_post t tr (i,m) (o,m') <-> join_succs curr_node pre tr i m o m'
+        ) ->
         body t = loop P ->
-        triple_gen a t n pre post tr i m o m'
+        triple_gen t curr_node pre tr i m o m'
     .
 
 
-    Definition valid_generated_triples   : Prop := 
+    (* each outgoing transition is associated with one more multiple triples *)
+    Definition valid_generated_triples  : Prop := 
         forall n , 
         reachable ag_aut n ->
-        forall pre post next_node , 
-        successor _ _ ag_aut next_node (pre,post) n  ->
+        forall pre post next_n,  successor _ _ ag_aut next_n (pre,post) n  ->
         forall tr i m o m',
-        exists t, triple_gen ag_aut t n pre post tr i m o m' /\ valid_triple t tr i m o m'
+        exists t, triple_gen t n pre tr i m o m' /\ valid_triple t tr i m o m'
     .
 
 End Reduction.
@@ -380,50 +439,64 @@ Abbreviation ag_aut_node := (a_aut_node * g_aut_node)%type.
 Abbreviation ag_aut_label  := (a_aut_label * g_aut_label)%type.
 
 Definition valid_contract_wit (C: Contract) (P: Program): Prop := 
-    (contract_setup C) (setup P tt) ->
-    forall t, 
-    run P t ->
+    (contract_setup C) (setup P) ->
+    forall i m o m' tr, 
+    run P (((i,m),(o,m'))::tr) ->
     forall i_tr m_tr o_tr m'_tr,
-    ((i_tr,m_tr),(o_tr,m'_tr)) = pgrm_trace_split t ->
-    forall a_p, language_wit sat_a (contract_assumes C) a_p (build_trace_history i_tr) -> 
-    exists ag_p, 
-        left_proj ag_p = a_p /\
-        language_wit sat_ag (ag_aut C) ag_p (build_trace_history t)
+    ((i_tr,m_tr),(o_tr,m'_tr)) = pgrm_trace_split tr ->
+    
+    forall a_p a_curr_trans a_next_node, 
+        language_wit sat_a (contract_assumes C) ((a_curr_trans,a_next_node)::a_p) (build_trace_history (i::i_tr)) -> 
+
+    exists ag_p, left_proj ag_p = a_p /\        
+    exists ag_curr_trans ag_next_node, 
+        language_wit sat_ag (ag_aut C) ((ag_curr_trans, ag_next_node)::ag_p) (build_trace_history (((i,m),(o,m'))::tr)) 
+        (* /\ (fst ag_curr_trans i_tr i <-> a_curr_trans i_tr i) *)
 .
 
 Lemma valid_contract_wit_valid C P : valid_contract_wit C P -> valid_contract C P.
 Proof.
-    intros  Hvalid_wit Hvalid_setup t Hrun i_tr m_tr [o_tr m'_tr] Hsplit Ha_lang.
-    destruct Ha_lang as (a_path & Ha_path & Ha_path_valid).
-    specialize (Hvalid_wit Hvalid_setup t Hrun i_tr m_tr o_tr m'_tr Hsplit a_path (conj Ha_path Ha_path_valid))
-         as (ag_path & Hag_p_a & Hag_path & Hag_path_valid).
-    exists (right_proj ag_path); split.
-    - now apply path_right_proj in Hag_path.
-    - eapply valid_right_proj  with  (sat:= sat_g) (transf:=id) in Hag_path_valid.
-        + replace (map fst (right_proj ag_path)) with (map snd (map fst ag_path)).
-            ++ now rewrite map_id in Hag_path_valid.
-            ++ clear. induction ag_path; [reflexivity|simpl; f_equal; apply IHag_path].
-        + intros * Hsat_ag. red in Hsat_ag. destruct b as [t'  ([i m] & [o m'])]. now apply Hsat_ag. 
+    intros  Hvalid_wit Hvalid_setup tr Hrun i_tr m_tr [o_tr m'_tr] Hsplit Ha_lang.
+    destruct Ha_lang as (a_path & Ha_path & Ha_path_valid). destruct a_path as [|[a_curr_label a_next_node] a_path].
+    -   (* empty path -> empty trace -> trivially sat *)
+        cbn in Ha_path_valid. inversion Ha_path_valid. symmetry in H; apply -> build_trace_history_iff_h_nil in H. subst. destruct tr eqn:X;[easy|].
+        destruct p as [[i m] [o m']].
+        pose proof  pgrm_trace_split_cons p0 i o m m'. now rewrite H in Hsplit. 
+
+    - destruct tr as [|[[i m] [o m']] tr];[easy|]. 
+        pose proof Hsplit as Hsplit'.
+        apply pgrm_trace_split_inv in Hsplit as (i_tl & m_tl & o_tl & m'_tl & Hsplit & Heq1 & Heq2 & Heq3 & Heq4); subst.
+    
+        specialize (Hvalid_wit Hvalid_setup _ _ _ _ _ Hrun _ _ _ _ Hsplit _ _ _ (conj Ha_path Ha_path_valid))
+         as (ag_path & Hleft_proj & [a_curr_label' g_curr_label] & [a_next_node' g_next_node] & Hag_path_valid ). 
+         rewrite build_trace_history_cons in *.
+        inversion_clear Hag_path_valid as [Hag_path Hag_path_valid'];  cbn in *.
+        exists ((g_curr_label,g_next_node)::right_proj ag_path); split. 
+    
+        + now apply path_right_proj in Hag_path.
+        + apply valid_right_proj  with  (sat:= sat_g) (transf:=id) in Hag_path_valid'.
+            * cbn in *. inversion Hag_path_valid'; subst; cbn in *. rewrite map_id in H2. constructor; [|assumption].
+                replace (map fst (right_proj ag_path)) with (map snd (map fst ag_path));[assumption|].
+                clear. induction ag_path; [reflexivity|simpl; f_equal; apply IHag_path].
+
+            * intros * Hsat_ag. red in Hsat_ag. now destruct b as [tr' [[i0 m0 ] [o0 m'0]]].  
 Qed.
-
-
 
 Theorem correctness_aux P C: 
     valid_generated_triples P C -> 
     valid_contract_wit C P. 
 Proof.
-    intros Htriples Hvalid_setup tr Hrun. induction Hrun.
+    intros Htriples Hvalid_setup i m o m' tr. revert i m o m'. induction tr.  
 
-    - (* first instant  *) 
-        intros i_tr m_tr o_tr m'_tr Htr_split a_path Ha_lang.
+    - intros i m o m' Hrun. (* first instant  *) 
+        inversion Hrun; subst.
+        intros i_tr m_tr o_tr m'_tr Htr_split a_path a_curr_label a_next_node Ha_lang.
         inversion Htr_split; subst.
         rewrite build_trace_history_cons in Ha_lang |- *.
 
 
         (* get current a_aut transition *)
-        inversion Ha_lang as (Ha_path & Ha_path_valid) ;
-        destruct a_path as [ | [a_curr_label a_next_node] a_path]; [ inversion Ha_path_valid |].
-
+        inversion Ha_lang as (Ha_path & Ha_path_valid). 
         inversion Ha_path_valid as [|? ?  ? ? Ha_path_valid_prev Ha_curr_valid]; subst.
         destruct a_path; [|easy].
         
@@ -432,10 +505,10 @@ Proof.
 
         (* we now show we also have a transition in ag_aut from the initial node to (a_n,g_n) such that
         its right component g_postcond satisfy the program first postcondition  *)
-        assert (exists g_curr_label g_next_node, 
+         assert (exists g_curr_label g_next_node, 
             transition (ag_aut C) (init (a_aut C), init (g_aut C)) (a_curr_label,g_curr_label) (a_next_node, g_next_node) /\ 
-            g_curr_label nil (i,setup P tt) (o, m')
-        ) as (g_curr_label & g_next_node & [ag_aut_trans Hg_n]).
+           (join_succs C (init (a_aut C), init (g_aut C)) a_curr_label nil i (setup P) o m')
+        ) as (g_curr_label & g_next_node & [ag_aut_trans Hsuccs]).
         {
 
             (* we have a transition in ag_aut from the initial node to (a_n,g_n) *)
@@ -449,112 +522,103 @@ Proof.
             }
 
             exists g_curr_label, g_next_node; split; cbn; [assumption|].
-
                                
             assert (Hinitreach : reachable (ag_aut C) (init (a_aut C), init (g_aut C))) by now constructor.
-            destruct (Htriples _ Hinitreach a_curr_label g_curr_label (a_next_node,g_next_node) Hag_trans nil i (setup P tt) o m')
-                 as (t & Htriples_gen & Htriples_valid).
-            inversion_clear Htriples_gen as  [Ht_pre Ht_post Ht_body].
-
+            specialize (Htriples _ Hinitreach _ _ _ Hag_trans nil i (setup P) o m') as (t & Htriples_gen & Htriples_valid).
+            inversion_clear Htriples_gen as [Hpre Hpost Ht_body]. apply Hpost.
+           
             (* this gives us the postcondition *)
-            rewrite <- Ht_post; apply Htriples_valid; [|now rewrite Ht_body]. 
-            rewrite Ht_pre;  cbn; split; [|assumption]. now constructor.
+            apply Htriples_valid; [|now rewrite Ht_body]. 
+            rewrite Hpre; cbn; split; [|assumption]. now constructor.
         }
 
-        exists (((a_curr_label,g_curr_label), (a_next_node,g_next_node))::nil). split; [reflexivity|].
-
-        split.
-        *  exact (path_transition _ _ _ _ _ _ ag_aut_trans).
-        *  assert (Hag_sat : sat_ag (a_curr_label, g_curr_label) (nil, ((i,setup P tt,(o, m')))))
-                by easy.
-            exact (valid_cons _ _ _ _ _ _ _ (valid_nil _ _ _) Hag_sat).
-
-
-    -  (* nth instant *)
-        intros i_tr m_tr o_tr m'_tr Htr_split a_path Ha_lang. 
-        apply (pgrm_trace_split_inv ( (prev_i, prev_m, (prev_o, m)) :: tr) i m o m' i_tr m_tr o_tr m'_tr) in Htr_split 
-            as  (i_tr' & m_tr' & o_tr' & m'_tr' & Htr_split & Hit & Hmt & Hotr & Hmtr); subst.
-        rename i_tr' into i_tr, o_tr' into o_tr, m_tr' into m_tr;
-        rewrite build_trace_history_cons in Ha_lang |- *.
+        exists nil. split; [now constructor|]. inversion Hsuccs as [a_curr_label' g_curr_label' [a_next_node' g_next_node'] ag_succ Ha_label_equiv Hg].
         
-        (* get current a_aut transition *)
-        inversion Ha_lang as (Ha_curr_path & Ha_curr_path_valid) ;
-        destruct a_path as [ | [a_curr_label a_next_node] a_path]; [ inversion Ha_curr_path_valid |]. 
+        (* ag_succ is the same path as ag_aut_trans *)
+        assert (Heq: (a_curr_label',g_curr_label') = (a_curr_label, g_curr_label) /\ (a_next_node', g_next_node') = (a_next_node, g_next_node)) by admit.
+        destruct Heq as [H1 H2]; inversion H1; inversion H2; subst.
+
+        exists (a_curr_label, g_curr_label), (a_next_node,g_next_node). split; [now constructor|]; constructor; [now constructor|now split].
+
+    - intros i m o m' Hrun.  (* nth instant *)
+        inversion Hrun as [|? ? ? ? ? ? ? ? Hrun' Hloop]; subst.
+        intros i_tr m_tr o_tr m'_tr Htr_split a_path a_curr_label a_next_node Ha_lang.
+        apply pgrm_trace_split_inv in Htr_split
+            as  (i_tr' & m_tr' & o_tr' & m'_tr' & Htr_split & Hit & Hmt & Hotr & Hmt').
+        inversion Hit; inversion Hmt; inversion Hotr; inversion Hmt'; subst; clear H H0 H1 H2;
+        rename i_tr' into i_tr, m_tr' into m_tr, o_tr' into o_tr, m'_tr' into m'_tr.
         
-        assert (Ha_lang_prev : language_wit sat_a (contract_assumes C) a_path (build_trace_history i_tr) ) by
-        now apply language_prefix_closed with (h := (a_curr_label, a_next_node)) (a :=(i_tr, i) ).
+        do 2 rewrite build_trace_history_cons in  *.
+        
+        inversion Ha_lang as [Ha_path Ha_valid]; inversion Ha_valid as [|? ? ? ? Ha_prev_valid Ha_curr X Y ]; subst.
+        
+        pose proof language_prefix_closed _ _ _ _ _ _ _ _ _ Ha_lang as Ha_lang_prev;
+        inversion Ha_lang_prev as [Ha_path_prev _].
 
-        inversion Ha_curr_path_valid as [|? ?  ? ? Ha_path_valid_prev Ha_curr_valid]; subst.
-
-    
+        destruct a_path as [|[a_prev_label a_curr_node] a_path];[easy|]. 
+        
         (* our induction hypothesis gives us a path in the product automaton 
             that contains the path from the assumption automaton, but with one less transition
             such that the trace up to the previous instant is valid
         *)
-        specialize (IHHrun _ _ _ _ Htr_split a_path Ha_lang_prev); clear Ha_lang_prev; move IHHrun at bottom;
-        destruct IHHrun as (ag_path & Hag_path_left_a & Hag_lang).
-        rewrite build_trace_history_cons  in *.
-
-        destruct ag_path as [|((a_prev_label & g_prev_label) & a_curr_node & g_curr_node) ag_path]; [now inversion Hag_lang|]; subst.
-
-        inversion Ha_curr_path as [|?|? ? ? ? ? Ha_path Ha_trans X]; subst.
+        specialize (IHtr _ _ _ _ Hrun' _ _ _ _ Htr_split); rewrite build_trace_history_cons in IHtr.
+        specialize (IHtr _ _ _ Ha_lang_prev) as (ag_path & Hag_path_left & (a_prev_label', g_prev_label) & (a_curr_node', g_curr_node) & Hag_lang_prev).
+        rewrite build_trace_history_cons in *.
 
 
-        apply (pgrm_trace_split_inv tr prev_i prev_m prev_o m i_tr m_tr o_tr) in Htr_split as 
-        (i_tr' & m_tr' & o_tr' & m'_tr'' & Htr_split & Hit & Hmt & Hot & Hm't); subst;
-        rename i_tr' into i_tr, o_tr' into o_tr, m_tr' into m_tr, m'_tr'' into m'_tr'; rewrite build_trace_history_cons in *;
-        cbn in *. 
+        inversion Hag_lang_prev as [Hag_path_prev Hag_valid_prev]; cbn in *.
+        pose proof valid_prefix_closed _ _ _ _ _ _ _ Hag_valid_prev as Hag_valid_prev_all.
+
+
+    (* because automata are deterministic, we have prev_label' = a_prev_label and a_curr_node' = a_curr_node *)
+        assert (a_prev_label' = a_prev_label /\ a_curr_node' = a_curr_node) as [H1 H2]. {
+            pose proof path_left_proj _ _ _ _ _ _ _ _ Hag_path_prev as H; cbn in H.
+            inversion Ha_path_prev.
+            -  inversion H;[|now rewrite <- H3, <- H7 in Hag_path_left]. subst. admit.
+            
+            - inversion H;[now rewrite <- H3, <- H8 in Hag_path_left|].
+                rewrite <- H3, <- H8 in Hag_path_left; inversion Hag_path_left; subst. 
+                admit.
+        } 
+
+        subst.
+
+        assert (Hag_curr_reach: reachable (ag_aut C) (a_curr_node, g_curr_node)) by (constructor 2; eauto).
+
+        pose proof ag_aut_complete _ _ Hag_curr_reach as ([a_curr_label' g_curr_label] & ag_next_node & Hag_trans).
+        inversion Hag_trans as [Ha_trans' Hg_trans]. 
+
+        inversion Ha_path as [X|?|? ? ? ? ?  _ Ha_trans]; subst. cbn in Ha_trans', Hg_trans.
+
+        assert (a_curr_label' = a_curr_label /\ a_next_node = fst ag_next_node) as [H1 H2]  by admit; subst. 
         
+        specialize (Htriples _ Hag_curr_reach _ _ _ Hag_trans ((prev_i, prev_m, (prev_o, m)) :: tr) i m o m') as (t & Htriple_gen & Hvalid_triple).
+        destruct Htriple_gen as [Ht_pre Ht_post Ht_body ].
 
-        inversion Hag_lang as [Hag_path Hag_path_valid] ; subst;
-            inversion Hag_path_valid as [X Hcontra | [tr'  [[prev_i' prev_m'] prev_o']] prev_ag_path ag_trans ag_m Hag_valid_prev_tr Hag_trans Hag_prev_path H_hist]; subst.
-
-        cbn in Hag_trans; destruct Hag_trans as [ Ha_prev_valid Hg_prev_valid ].
-        
-
-        (* current node in the product is reachable *)
-        assert (Hag_curr_reach: reachable (ag_aut C) (a_curr_node, g_curr_node)). {
-                right. exists (a_prev_label, g_prev_label). 
-                now exists ag_path.
+        assert (Ha_curr_sat : a_curr_label (trace_to_input_trace ((prev_i, prev_m, (prev_o, m)) :: tr)) i). {
+            unfold trace_to_input_trace in Ht_pre |- * ; rewrite pgrm_trace_split_cons in Ht_pre |- *; cbn in Ht_pre |- *; subst. 
+            now inversion Htr_split.
         }
 
-        (* we have a transition in ag_aut from the current node to the next whose left projection is a_curr_node  *)
-        assert (exists (g_curr_label : g_aut_label) g_next_node,
-                        transition (ag_aut C) (a_curr_node,g_curr_node) (a_curr_label, g_curr_label) (a_next_node,g_next_node))
-        as (g_curr_label & g_next_node & Hag_trans_next).
+        assert (Hw_join :join_succs C (a_curr_node, g_curr_node) a_curr_label ((prev_i, prev_m, (prev_o, m)) :: tr) i m o m' -> g_curr_label ((prev_i, prev_m, (prev_o, m)) :: tr) (i, m) (o, m')).
         {
-            (* this is because the product contains a path in g_aut g_curr_node and g_aut is complete *)
-            assert (Hg_reach_m : reachable (g_aut C) g_curr_node) by (now apply reachable_right_proj in Hag_curr_reach).
-            pose proof (g_aut_complete _ _ Hg_reach_m) as (g_curr_label & g_next_node & Hg_trans). 
-            now  exists g_curr_label, g_next_node.
+            intros Hj. inversion Hj.  
+            (* as we are deterministic, post' must be g_curr_label *) 
+            admit.            
         }
 
-        cbn in  Hag_trans_next; destruct Hag_trans_next as [ _ Hg_trans ].
+        exists (((a_prev_label, g_prev_label),(a_curr_node,g_curr_node))::ag_path); split; [reflexivity|].
+        exists (a_curr_label, g_curr_label), ag_next_node. split; [now constructor|]; cbn. constructor; [assumption|]; constructor; [assumption|]; cbn.
+        apply Hw_join; apply Ht_post; apply Hvalid_triple; [|now rewrite Ht_body]. apply Ht_pre; split; [|assumption].
 
-        assert (Hag_succ: successor _ _ (ag_aut C) (a_next_node, g_next_node) (a_curr_label, g_curr_label) (a_curr_node, g_curr_node)) by easy. 
-
-
-        specialize (Htriples  (a_curr_node, g_curr_node) Hag_curr_reach a_curr_label g_curr_label (a_next_node,g_next_node) Hag_succ ((prev_i, prev_m, (prev_o, m)) :: tr) i m o m') 
-            as (t & Htriple_gen & Hvalid_triple);
-        destruct Htriple_gen as [Hcurr_t_pre Hcurr_t_post Hcurr_t_body].
-
-        exists (((a_curr_label,g_curr_label), (a_next_node,g_next_node))::((a_prev_label,g_prev_label), (a_curr_node,g_curr_node))::ag_path).
-        split; [reflexivity|]; split; cbn.
-
-        + now constructor.
-        + constructor; [now constructor|]; split; cbn.
-            * unfold private_to_input_trace; rewrite pgrm_trace_split_cons; cbn; subst.
-                now  inversion_clear Htr_split; cbn.
-                
-            *  rewrite <- Hcurr_t_post.
-                apply Hvalid_triple; [|now rewrite Hcurr_t_body ]; clear Hcurr_t_body.
-                rewrite Hcurr_t_pre. split.
-                -- inversion Hag_path as [X|? ? Hprev_trans X |ag_prev_node ? ag_prev_label ? ag_path' Hprev_path Hprev_trans X]; subst.
-                    ++ now constructor 2 with (precond:=(a_prev_label, g_prev_label)) (prev_n:=(init (ag_aut C))).
-                    ++ now constructor 2 with (precond:=(a_prev_label, g_prev_label)) (prev_n:=(ag_prev_node)).                    
-                -- unfold private_to_input_trace; rewrite pgrm_trace_split_cons; cbn; subst.
-                    now inversion_clear Htr_split; cbn.
-Qed.
+        inversion Hag_path_prev; subst.
+        + apply (join_preds_cons _ _ _ _ (init (ag_aut C)) (a_prev_label,g_prev_label) (a_curr_node,g_curr_node)).
+            * apply H0.
+            * cbn. inversion Hag_valid_prev; subst. now inversion H5.
+        + apply (join_preds_cons _ _ _ _ m0 (a_prev_label,g_prev_label) (a_curr_node,g_curr_node)).
+            * apply H3.
+            * cbn. inversion Hag_valid_prev; subst. apply H6.
+Admitted.
 
 
 Corollary correctness P C : 
